Large cleanup of the Bags and ProcessScheduler codebases

ADTExamples/QueryStructure/ProcessScheduler/AdditionalLemmas.v
@@ -2,7 +2,7 @@ Require Import Ensembles List Coq.Lists.SetoidList Program
         Common Computation.Core
         ADTNotation.BuildADTSig ADTNotation.BuildADT
         GeneralBuildADTRefinements QueryQSSpecs QueryStructure
-        SetEq.
+        SetEq Omega.
 Require Export EnsembleListEquivalence.
 
 Unset Implicit Arguments.
@@ -26,7 +26,7 @@ Section AdditionalDefinitions.
       match pred a with
         | left _  => true
         | right _ => false
-      end.
+      end. (* TODO: Use this *)
 
   Definition Box {A: Type} (x: A) := [x].
 
@@ -43,10 +43,59 @@ Section AdditionalDefinitions.
     forall (a: A), @eq B (f a) (g a).
 End AdditionalDefinitions.
 
+Section AdditionalNatLemmas.
+  Lemma le_r_le_max : 
+    forall x y z,
+      x <= z -> x <= max y z.
+  Proof.
+    intros x y z;
+    destruct (Max.max_spec y z) as [ (comp, eq) | (comp, eq) ]; 
+    rewrite eq;
+    omega.
+  Qed.
+
+  Lemma le_l_le_max : 
+    forall x y z,
+      x <= y -> x <= max y z.
+  Proof.
+    intros x y z. 
+    rewrite Max.max_comm.
+    apply le_r_le_max.
+  Qed.
+End AdditionalNatLemmas.
+
 Section AdditionalLogicLemmas.
   Lemma or_false :
     forall (P: Prop), P \/ False <-> P.
   Proof.
+    tauto.
+  Qed.
+
+  Lemma false_or :
+    forall (P Q: Prop),
+      (False <-> P \/ Q) <-> (False <-> P) /\ (False <-> Q).
+  Proof.
+    tauto.
+  Qed.
+
+  Lemma false_or' :
+    forall (P Q: Prop),
+      (P \/ Q <-> False) <-> (False <-> P) /\ (False <-> Q).
+  Proof.
+    tauto.
+  Qed.
+
+  Lemma equiv_false :
+    forall P,
+      (False <-> P) <-> (~ P).
+  Proof. 
+    tauto.
+  Qed.
+
+  Lemma equiv_false' :
+    forall P,
+      (P <-> False) <-> (~ P).
+  Proof. 
     tauto.
   Qed.
 
@@ -56,6 +105,24 @@ Section AdditionalLogicLemmas.
     split; intros; symmetry; assumption.
   Qed.
 End AdditionalLogicLemmas.
+
+Section AdditionalBoolLemmas.
+  Lemma collapse_ifs_dec :
+    forall P (b: {P} + {~P}),
+      (if (if b then true else false) then true else false) =
+      (if b then true else false).
+  Proof.
+    destruct b; reflexivity.
+  Qed.
+
+  Lemma collapse_ifs_bool :
+    forall (b: bool),
+      (if (if b then true else false) then true else false) =
+      (if b then true else false).
+  Proof.
+    destruct b; reflexivity.
+  Qed.
+End AdditionalBoolLemmas.
 
 Section AdditionalEnsembleLemmas.
   Lemma weaken :
@@ -74,6 +141,34 @@ Section AdditionalListLemmas.
       (map (fun x => x) seq) = seq.
   Proof.
     intros A seq; induction seq; simpl; congruence.
+  Qed.
+
+  Lemma in_nil_iff :
+    forall {A} (item: A),
+      List.In item [] <-> False.
+  Proof.
+    intuition.
+  Qed.
+
+  Lemma in_not_nil :
+    forall {A} x seq,
+      @List.In A x seq -> seq <> nil.
+  Proof.
+    intros A x seq in_seq eq_nil.
+    apply (@in_nil _ x).
+    subst seq; assumption.
+  Qed.
+
+  Lemma in_seq_false_nil_iff :
+    forall {A} (seq: list A),
+      (forall (item: A), (List.In item seq <-> False)) <-> 
+      (seq = []).
+  Proof.
+    intros.
+    destruct seq; simpl in *; try tauto.
+    split; intro H.
+    exfalso; specialize (H a); rewrite <- H; eauto.
+    discriminate.
   Qed.
 
   Lemma filter_comm :
@@ -205,6 +300,25 @@ Section AdditionalListLemmas.
     trivial.
   Qed.
 
+  Definition flatten {A} seq := List.fold_right (@app A) [] seq.
+
+  Lemma in_flatten_iff :
+    forall {A} x seqs, 
+      @List.In A x (flatten seqs) <-> 
+      exists seq, List.In x seq /\ List.In seq seqs.
+  Proof.
+    intros; unfold flatten.
+    induction seqs; simpl. 
+
+    firstorder.
+    rewrite in_app_iff.
+    rewrite IHseqs.
+
+    split.
+    intros [ in_head | [seq (in_seqs & in_seq) ] ]; eauto.
+    intros [ seq ( in_seq & [ eq_head | in_seqs ] ) ]; subst; eauto.
+  Qed.
+
   Lemma flatten_filter :
     forall {A} (seq: list (list A)) pred, 
       List.filter pred (flatten seq) =
@@ -264,6 +378,20 @@ Section AdditionalListLemmas.
     apply IH; firstorder.
   Qed.
 
+  Lemma foldright_compose :
+    forall {TInf TOutf TAcc} 
+           (g : TOutf -> TAcc -> TAcc) (f : TInf -> TOutf) 
+           (seq : list TInf) (init : TAcc),
+      List.fold_right (compose g f) init seq =
+      List.fold_right g init (List.map f seq).
+  Proof.
+    intros; 
+    induction seq; 
+    simpl; 
+    [  | rewrite IHseq ];
+    reflexivity.
+  Qed.            
+
   Lemma flatten_nils :
     forall {A} (seq: list (list A)),
       flatten (List.map (fun _ => []) seq) = @nil A.
@@ -284,6 +412,20 @@ Section AdditionalListLemmas.
       @flatten A (head :: tail) = head ++ flatten tail.
   Proof.
     intuition.
+  Qed.
+
+  Lemma in_map_unproject :
+    forall {A B} projection seq,
+    forall item,
+      @List.In A item seq ->
+      @List.In B (projection item) (List.map projection seq).
+  Proof.
+    intros ? ? ? seq;
+    induction seq; simpl; intros item in_seq.
+
+    trivial.
+    destruct in_seq;
+      [ left; f_equal | right ]; intuition.
   Qed.
 End AdditionalListLemmas.
 
@@ -352,43 +494,10 @@ Ltac refine_eq_into_ret :=
         apply (refine_eqA_into_ret _)
   end.
 
-Ltac hone_observer' name :=
-  hone constructor name using _;
-  [ simpl;
-    unfold refine;
-    intros;
-    unfold Query_For, Query_Where,
-    Query_In, Query_Return, qsHint,
-    In, qsSchemaHint;
-    constructor;
-    intros;
-    constructor;
-    intros;
-    repeat subst;
-    constructor;
-    generalize_all | ].
+Ltac prove_observational_eq :=
+  lazy; intuition (eauto using collapse_ifs_bool, collapse_ifs_dec; eauto with *).
 
-(* TODO: This could probably inconjunction with pull_definition to
-avoid the case disjunction in there, but I'm not sure how to allow
-unification to proceed: it seems that only a let inside of the
-instantiation pattern will do.  *)
-Ltac uncurry_evar :=
-  instantiate (1 := (fun x => _ (fst x) (snd x)));
-  simpl.
-
-Ltac pull_definition :=
-  match goal with
-    | [ |- ?f (?db1, (?db2, ?db3)) ?params = ret ?body ] =>
-      instantiate (1 := fun db params => let (db1, db23) := db in let (db2, db3) := db23 in ret _)
-    | [ |- ?f (?db1, ?db2) ?params = ret ?body ] =>
-      instantiate (1 := fun db params => let (db1, db2) := db in ret _)
-    | [ |- ?f ?db ?params = ret ?body ] =>
-      instantiate (1 := fun db params => ret (_ db params))
-  end;
-  simpl;
-  exists.
-
-Section AdditionalQueryLemmas.
+Section AdditionalQueryLemmas. (* TODO: Kill the two following lemmas. They are outdated now. :'( *)
   Lemma refine_ensemble_into_list_with_extraction :
     forall {A B: Type} (la: list A) (ens: A -> Prop) (lb: list B)
            (cond_prop: A -> Prop) (cond: A -> bool)
