ADTExamples/QueryStructure/Bags/BagsOfTuples.v
@@ -1,0 +1,132 @@
+Require Export Bags TreeBags ListBags Tuple Heading List Program.
+Require Import String_as_OT.
+Require Import Bool String OrderedTypeEx.
+
+Unset Implicit Arguments.
+
+Definition TSearchTermMatcher (heading: Heading) := (@Tuple heading -> bool).
+
+Definition SearchTermsCollection heading :=
+  list (TSearchTermMatcher heading).
+
+Fixpoint MatchAgainstSearchTerms 
+         {heading: Heading}
+         (search_terms : SearchTermsCollection heading) (item: Tuple) :=
+  match search_terms with
+    | []                     => true
+    | is_match :: more_terms => (is_match item) && MatchAgainstSearchTerms more_terms item
+  end.
+
+Definition HasDecidableEquality (T: Type) :=
+  forall (x y: T), {x = y} + {x <> y}.
+
+Definition TupleEqualityMatcher 
+           {heading: Heading} 
+           (attr: Attributes heading)
+           (value: Domain heading attr) 
+           {eq_dec: HasDecidableEquality (Domain heading attr)} : TSearchTermMatcher heading :=
+  fun tuple => 
+    match eq_dec (tuple attr) value with
+      | in_left  => true
+      | in_right => false
+    end.
+
+Instance TupleListAsBag (heading: Heading) :
+  Bag (list (@Tuple heading)) (@Tuple heading) (SearchTermsCollection heading).
+Proof.
+  apply (ListAsBag [] (@MatchAgainstSearchTerms heading)); eauto.
+Defined.
+
+Require Import FMapAVL.
+
+Module NatIndexedMap := FMapAVL.Make Nat_as_OT.
+Module StringIndexedMap := FMapAVL.Make String_as_OT.
+
+Module NatTreeBag := TreeBag NatIndexedMap.
+Module StringTreeBag := TreeBag StringIndexedMap.
+
+Definition NatTreeType TSubtree TSubtreeSearchTerm heading subtree_as_bag := 
+  (@NatTreeBag.IndexedBag 
+     TSubtree 
+     (@Tuple heading) 
+     TSubtreeSearchTerm 
+     subtree_as_bag).
+
+Definition StringTreeType TSubtree TSubtreeSearchTerm heading subtree_as_bag := 
+  (@StringTreeBag.IndexedBag 
+     TSubtree 
+     (@Tuple heading) 
+     TSubtreeSearchTerm
+     subtree_as_bag).
+
+Definition cast {T1 T2: Type} (eq: T1 = T2) (x: T1) : T2.
+Proof.
+  subst; auto.
+Defined.
+
+Record ProperAttribute {heading} :=
+  {
+    Attribute: Attributes heading; 
+    ProperlyTyped: { Domain heading Attribute = nat } + { Domain heading Attribute = string }
+  }.
+
+Fixpoint NestedTreeFromAttributes'
+         heading 
+         (indexes: list (@ProperAttribute heading)) 
+         {struct indexes}: (@BagPlusBagProof (@Tuple heading)) :=
+  match indexes with
+    | [] => 
+      {| BagType        := list (@Tuple heading);
+         SearchTermType := SearchTermsCollection heading |}
+    | proper_attr :: more_indexes => 
+      let attr := @Attribute heading proper_attr in
+      let (t, st, bagproof) := NestedTreeFromAttributes' heading more_indexes in
+      match (@ProperlyTyped heading proper_attr) with
+        | left  eq_nat    => 
+          {| BagType        := NatTreeType    t st heading bagproof (fun x => cast eq_nat    (x attr));
+             SearchTermType := option nat    * st |}
+        | right eq_string => 
+          {| BagType        := StringTreeType t st heading bagproof (fun x => cast eq_string (x attr));
+             SearchTermType := option string * st |}
+      end
+    end.
+
+Definition CheckType {heading} (attr: Attributes heading) (rightT: _) :=
+  {| Attribute := attr; ProperlyTyped := rightT |}.
+
+Ltac autoconvert func :=
+  match goal with 
+    | [ src := cons ?head ?tail |- list _ ] =>
+      refine (func head _ :: _);
+        [ solve [ eauto with * ] | clear src;
+                            set (src := tail);
+                            autoconvert func ]
+    | [ src := nil |- list _ ] => apply []
+    | _ => idtac
+  end.
+
+Ltac mkIndex heading attributes :=
+  set (src := attributes);
+  assert (list (@ProperAttribute heading)) as decorated_source by autoconvert (@CheckType heading);
+  apply (NestedTreeFromAttributes' heading decorated_source).
+
+(* Example use:
+Require Import Beatles.
+
+Definition SampleIndex : @BagPlusBagProof (@Tuple AlbumHeading).
+Proof.
+  mkIndex AlbumHeading [Year; UKpeak; Name].
+Defined.
+
+Definition IndexedAlbums :=
+  List.fold_left binsert FirstAlbums (@bempty _ _ _ (BagProof SampleIndex)).
+
+Eval simpl in (SearchTermType SampleIndex).
+Time Eval simpl in (bfind IndexedAlbums (Some 3, (None, (None, [])))).
+Time Eval simpl in (bfind IndexedAlbums (Some 3, (Some 1, (None, [])))).
+Time Eval simpl in (bfind IndexedAlbums (Some 3, (Some 1, (Some "With the Beatles", [])))).
+Time Eval simpl in (bfind IndexedAlbums (None, (None, (Some "With the Beatles", [])))).
+Time Eval simpl in (bfind IndexedAlbums (None, (None, (None, [TupleEqualityMatcher (eq_dec := string_dec) Name "With the Beatles"])))).
+
+(*Time Eval simpl in (@bfind _ _ _ (BagProof _ SampleIndex) IndexedAlbums (Some 3, (Some 1, (None, @nil (TSearchTermMatcher AlbumHeading))))).*)
+*)
