ADTExamples/QueryStructure/Bags/CachingBags.v
@@ -1,0 +1,290 @@
+Require Export Bags.
+Require Import AdditionalLemmas.
+
+Unset Implicit Arguments.
+
+Definition IsCacheable
+           {TItem TAcc}
+           (initial_value: TAcc)
+           (cache_updater: TItem -> TAcc -> TAcc) :=
+  forall seq1 seq2,
+    SetEq seq1 seq2 ->
+    (List.fold_right cache_updater initial_value seq1 =
+     List.fold_right cache_updater initial_value seq2).
+
+Record CachingBag 
+       {TBag TItem TSearchTerm: Type} 
+       {bag_bag: Bag TBag TItem TSearchTerm} 
+       {TCachedValue: Type}
+       {initial_cached_value: TCachedValue}
+       {cache_updater: TItem -> TCachedValue -> TCachedValue} 
+       {cache_updater_cacheable: IsCacheable initial_cached_value cache_updater} :=
+  { 
+    cbag:          TBag;
+    ccached_value: TCachedValue;
+    
+    cfresh_cache:  List.fold_right cache_updater initial_cached_value (benumerate cbag) = ccached_value
+  }.
+
+(* Note: The caching interface provides the initial_cached_value
+         parameter to allow implementations to gracefully handle empty
+         caches. Should an empty/non-empty distinction be needed,
+         initial_cached_value can be set to None, and TCachedValue
+         replaced by an option type. *)
+
+Lemma binsert_enumerate_SetEq {TContainer TItem TSearchTerm} (bag: Bag TContainer TItem TSearchTerm):
+  forall inserted container,
+    SetEq 
+      (benumerate (binsert container inserted))
+      (inserted :: (benumerate container)).
+Proof.
+  unfold SetEq; intros; simpl.
+  setoid_rewrite or_comm; setoid_rewrite eq_sym_iff. 
+  apply binsert_enumerate. 
+Qed.
+
+Lemma benumerate_empty_eq_nil {TContainer TItem TSearchTerm} (bag: Bag TContainer TItem TSearchTerm):
+  (benumerate bempty) = nil. 
+Proof.
+  pose proof (benumerate_empty) as not_in;
+  unfold BagEnumerateEmpty in not_in.
+  destruct (benumerate bempty) as [ | item ? ]; 
+    simpl in *;
+    [ | exfalso; apply (not_in item) ];
+    eauto.
+Qed.
+
+Instance CachingBagAsBag 
+         {TBag TItem TSearchTerm: Type} 
+         {bag_bag: Bag TBag TItem TSearchTerm} 
+         {TCachedValue: Type}
+         {initial_cached_value: TCachedValue} 
+         {cache_updater: TItem -> TCachedValue -> TCachedValue} 
+         {cache_updater_cacheable: IsCacheable initial_cached_value cache_updater}
+         : Bag (@CachingBag TBag TItem TSearchTerm bag_bag 
+                            TCachedValue initial_cached_value cache_updater
+                            cache_updater_cacheable) 
+               TItem 
+               TSearchTerm :=
+  {| 
+    bempty                         := {| cbag          := @bempty _ _ _ bag_bag; 
+                                         ccached_value := initial_cached_value |};
+    bstar                          := @bstar _ _ _ bag_bag;
+    bfind_matcher search_term item := bfind_matcher search_term item;
+
+    benumerate container        := benumerate container.(cbag);
+    bfind container search_term := bfind container.(cbag) search_term; 
+    binsert container item      := {| cbag          := binsert container.(cbag) item;
+                                      ccached_value := cache_updater item container.(ccached_value) |} 
+  |}.
+Proof.    
+  unfold BagInsertEnumerate; simpl; intros. apply binsert_enumerate.
+  unfold BagEnumerateEmpty;  simpl; intros; apply benumerate_empty.
+  unfold BagFindStar;        simpl; intros; apply bfind_star.
+  unfold BagFindCorrect;     simpl; intros; apply bfind_correct.
+
+  Grab Existential Variables.
+
+  rewrite (cache_updater_cacheable _ _ (binsert_enumerate_SetEq bag_bag _ _));
+  simpl; setoid_rewrite cfresh_cache; reflexivity.
+
+  rewrite benumerate_empty_eq_nil; reflexivity.
+Defined.
+
+Section CacheableFunctions.
+  Section Generalities.
+    Lemma projection_cacheable :
+      forall {TItem TCacheUpdaterInput TCachedValue} 
+             (projection: TItem -> TCacheUpdaterInput)
+             (cache_updater: TCacheUpdaterInput -> TCachedValue -> TCachedValue)
+             (initial_value: TCachedValue),
+        IsCacheable initial_value cache_updater -> 
+        IsCacheable initial_value (compose cache_updater projection).
+      Proof.
+        unfold IsCacheable.
+        intros * is_cacheable * set_eq. 
+        rewrite !foldright_compose;
+          apply is_cacheable;
+          rewrite set_eq;
+          reflexivity.
+      Qed.
+
+      Definition AddCachingLayer
+                 {TBag TItem TSearchTerm: Type} 
+                 (bag: Bag TBag TItem TSearchTerm)
+                 {TCacheUpdaterInput TCachedValue: Type}
+                 (cache_projection: TItem -> TCacheUpdaterInput) 
+                 (initial_cached_value: TCachedValue)
+                 (cache_updater: TCacheUpdaterInput -> TCachedValue -> TCachedValue) 
+                 (cache_updater_cacheable: IsCacheable initial_cached_value cache_updater) :=
+        {|
+          BagType       :=  @CachingBag TBag TItem TSearchTerm 
+                                        bag TCachedValue initial_cached_value 
+                                        (compose cache_updater cache_projection) 
+                                        (projection_cacheable cache_projection 
+                                                              cache_updater 
+                                                              initial_cached_value 
+                                                              cache_updater_cacheable);
+          SearchTermType := TSearchTerm;
+          BagProof       := _
+        |}.
+
+      Definition CacheImplementationEnsures
+                 {TCacheUpdaterInput TCachedValue}
+                 cache_property
+                 (cache_updater: TCacheUpdaterInput -> TCachedValue -> TCachedValue) 
+                 (initial_value: TCachedValue) :=
+        forall seq (value: TCacheUpdaterInput),
+          cache_property seq value (List.fold_right cache_updater initial_value seq).
+
+      Definition ProjectedCacheImplementationEnsures
+                 {TItem TCacheUpdaterInput TCachedValue}
+                 cache_property
+                 (cache_updater: TCacheUpdaterInput -> TCachedValue -> TCachedValue) 
+                 (projection: TItem -> TCacheUpdaterInput)
+                 (initial_value: TCachedValue) :=
+        forall seq (item: TItem),
+          cache_property (List.map projection seq) (projection item) (List.fold_right (compose cache_updater projection) initial_value seq).
+
+      (* Formally equivalent to ProjectedCacheImplementationEnsures cache_property id initial_value *)
+
+      Lemma generalize_to_projection :
+        forall {TItem TCacheUpdaterInput TCachedValue} 
+               {cache_updater: TCacheUpdaterInput -> TCachedValue -> TCachedValue}
+               (projection: TItem -> TCacheUpdaterInput)
+               (initial_value: TCachedValue)
+               (cache_property: list TCacheUpdaterInput ->
+                                TCacheUpdaterInput -> TCachedValue -> Type),
+          (CacheImplementationEnsures          
+             cache_property cache_updater initial_value) ->
+          (ProjectedCacheImplementationEnsures
+             cache_property cache_updater projection initial_value).
+      Proof.
+        unfold CacheImplementationEnsures, ProjectedCacheImplementationEnsures;
+        intros * non_projected_proof *;
+        rewrite foldright_compose;
+        apply non_projected_proof.
+      Qed.
+  End Generalities.
+
+  Section MaxCacheable.
+    Definition IsMax m seq :=
+      (forall x, List.In x seq -> x <= m) /\ List.In m seq.
+
+    Require Import Setoid.
+    Add Parametric Morphism (m: nat) :
+      (IsMax m)
+        with signature (@SetEq nat ==> iff)
+          as IsMax_morphism.
+    Proof.
+      firstorder.
+    Qed.
+
+    Definition ListMax default seq :=
+      List.fold_right max default seq.
+
+    Lemma ListMax_correct_nil :
+      forall seq default,
+        seq = nil -> ListMax default seq = default.
+    Proof.
+      unfold ListMax; intros; subst; intuition.
+    Qed.
+    
+    Lemma ListMax_correct :
+      forall seq default,
+        IsMax (ListMax default seq) (default :: seq).
+    Proof.
+      unfold IsMax; 
+      induction seq as [ | head tail IH ]; 
+      intros; simpl.
+      
+      intuition.
+
+      specialize (IH default);
+        destruct IH as (sup & in_seq).
+
+      split. 
+
+      intros x [ eq | [ eq | in_tail ] ].
+      
+      apply le_r_le_max, sup; simpl; intuition.
+      apply le_l_le_max; subst; intuition.
+      apply le_r_le_max, sup; simpl; intuition.
+
+      destruct in_seq as [ max_default | max_in_tail ].
+
+      rewrite <- max_default, Max.max_comm;
+        destruct (Max.max_spec default head); 
+        intuition.
+
+      match goal with
+        | [ |- context[ max ?a ?b ] ] => destruct (Max.max_spec a b) as [ (comp & max_eq) | (comp & max_eq) ]
+      end; rewrite max_eq; intuition.
+    Qed.
+
+    Lemma Max_unique :
+      forall {x y} seq,
+        IsMax x seq ->
+        IsMax y seq -> 
+        x = y.
+    Proof.
+      unfold IsMax;
+      intros x y seq (x_sup & x_in) (y_sup & y_in);
+      specialize (x_sup _ y_in);
+      specialize (y_sup _ x_in);
+      apply Le.le_antisym; assumption.
+    Qed.
+
+    (* TODO: rename SetEq_append to SetEq_cons *)
+
+    (* TODO: find a cleaner way than destruct; discriminate *)
+    (* TODO: Look at reflexive, discriminate, congruence, absurd in more details *)
+    Lemma ListMax_cacheable :
+      forall initial_value,
+        IsCacheable initial_value max.
+    Proof.
+      unfold IsCacheable.
+
+      intros init seq1 seq2 set_eq;
+        apply (Max_unique (init :: seq1));
+        [ | setoid_rewrite (SetEq_append init set_eq) ];
+        apply ListMax_correct.
+    Qed.
+
+    Definition cached_max_gt_property seq value cached_max :=
+      List.In value seq -> S cached_max > value.
+
+    Lemma cached_max_gt :
+      forall default,
+        CacheImplementationEnsures cached_max_gt_property max default. 
+    Proof.
+      unfold CacheImplementationEnsures, cached_max_gt_property; 
+      intros;
+      destruct (ListMax_correct seq default) as (sup & _);
+      apply Gt.le_gt_S, sup;
+      simpl; auto.
+    Qed.
+
+    Lemma cached_max_gt_projected' {TItem} projection :
+      forall default,
+        ProjectedCacheImplementationEnsures (TItem := TItem) cached_max_gt_property max projection default.
+    Proof.
+      unfold ProjectedCacheImplementationEnsures.
+      unfold cached_max_gt_property.
+
+      intros;
+      apply (generalize_to_projection projection default cached_max_gt_property (cached_max_gt default));
+      trivial.
+    Qed.
+
+    Lemma cached_max_gt_projected : 
+      forall {A} projection,
+      forall default seq (item: A),
+        List.In item seq -> S (List.fold_right (compose max projection) default seq) > (projection item).
+    Proof.
+      intros;
+      apply (cached_max_gt_projected' projection);
+      apply (in_map_unproject); trivial.
+    Qed.
+  End MaxCacheable.
+End CacheableFunctions.
