ADTExamples/QueryStructure/Bags/ListBags.v
@@ -1,0 +1,68 @@
+Require Export Bags.
+Unset Implicit Arguments.
+
+Definition ListAsBag_bfind 
+           {TItem TSearchTerm: Type}
+           (matcher: TSearchTerm -> TItem -> bool) 
+           (container: list TItem) (search_term: TSearchTerm) :=
+  List.filter (matcher search_term) container.
+
+Definition ListAsBag_binsert 
+           {TItem: Type}
+           (container: list TItem) 
+           (item: TItem) :=
+  cons item container.
+
+Lemma List_BagInsertEnumerate :
+  forall {TItem: Type},
+  BagInsertEnumerate id (ListAsBag_binsert (TItem := TItem)).
+Proof.
+  firstorder.
+Qed.
+
+Lemma List_BagFindStar :
+  forall {TItem TSearchTerm: Type}
+         (star: TSearchTerm)
+         (matcher: TSearchTerm -> TItem -> bool)
+         (find_star: forall (i: TItem), matcher star i = true),
+  BagFindStar (ListAsBag_bfind matcher) id star.
+Proof.
+  intros;
+  induction container; simpl; 
+  [ | rewrite find_star, IHcontainer]; trivial.
+Qed.
+
+Lemma List_BagEnumerateEmpty :
+  forall {TItem: Type},
+    BagEnumerateEmpty id (@nil TItem).
+Proof.
+  firstorder.
+Qed.
+  
+Lemma List_BagFindCorrect :
+  forall {TItem TSearchTerm: Type}
+         (matcher: TSearchTerm -> TItem -> bool),
+         BagFindCorrect (ListAsBag_bfind matcher) matcher id.
+Proof.
+  firstorder.
+Qed.
+
+Instance ListAsBag
+         {TItem TSearchTerm: Type}
+         (star: TSearchTerm)
+         (matcher: TSearchTerm -> TItem -> bool)
+         (find_star: forall (i: TItem), matcher star i = true)
+: Bag (list TItem) TItem TSearchTerm :=
+  {| 
+    bempty := nil;
+    bstar  := star;
+    
+    benumerate := id;
+    bfind      := ListAsBag_bfind matcher;
+    binsert    := ListAsBag_binsert;
+    
+    binsert_enumerate := List_BagInsertEnumerate;
+    benumerate_empty  := List_BagEnumerateEmpty;
+    bfind_star        := List_BagFindStar star matcher find_star;
+    bfind_correct     := List_BagFindCorrect matcher
+  |}.
