ADTExamples/QueryStructure/Bags/TreeBags.v
@@ -1,0 +1,544 @@
+Require Export Bags.
+Require Import SetEqProperties FMapExtensions AdditionalLemmas.
+Require Import FMapInterface Coq.FSets.FMapFacts.
+
+Unset Implicit Arguments.
+
+Module TreeBag (Import M: WS).
+  Module Import BasicFacts := WFacts_fun E M.
+  Module Import BasicProperties := WProperties_fun E M.
+  Module Import MoreFacts := FMapExtensions_fun E M.
+
+  Definition TKey := key.
+
+  Definition IndexedTreeConsistency 
+             {TBag TItem TBagSearchTerm: Type}
+             {bags_bag: Bag TBag TItem TBagSearchTerm}
+             projection fmap :=
+    forall (key: TKey) (bag: TBag),
+      MapsTo key bag fmap -> 
+      forall (item: TItem),
+        List.In item (benumerate bag) ->
+        E.eq (projection item) key.
+
+  Record IndexedBag 
+         {TBag TItem TBagSearchTerm: Type} 
+         {bags_bag: Bag TBag TItem TBagSearchTerm} 
+         {projection} :=
+    { 
+      ifmap        : t TBag;
+      iconsistency : IndexedTreeConsistency projection ifmap
+    }.
+
+  Definition KeyFilter 
+             {TItem}
+             (key: TKey)
+             (projection: TItem -> TKey) :=
+    (fun x : TItem => if E.eq_dec (projection x) key then true else false).
+  
+  Lemma KeyFilter_beq :
+    forall {TItem} beq,
+      (forall x y, reflect (E.eq x y) (beq x y)) ->
+      (forall key projection (item: TItem), 
+         KeyFilter key projection item = beq (projection item) key).
+  Proof.
+    intros TItem beq spec key projection item.
+    specialize (spec (projection item) key).
+    unfold KeyFilter.
+    destruct spec as [ is_eq | neq ];
+    destruct (F.eq_dec _ _); intuition.
+  Qed.    
+
+  Lemma iconsistency_empty :
+    forall {TBag TItem TBagSearchTerm: Type} 
+           {bags_bag: Bag TBag TItem TBagSearchTerm} 
+           projection,
+      IndexedTreeConsistency projection (empty TBag).
+  Proof.
+      unfold IndexedTreeConsistency; 
+      intros; rewrite empty_mapsto_iff in *; exfalso; trivial.
+  Qed.
+
+  Lemma consistency_key_eq :
+    forall {TBag TItem TBagSearchTerm},
+    forall bags_bag (projection: TItem -> TKey),
+    forall (indexed_bag: @IndexedBag TBag TItem TBagSearchTerm bags_bag projection),
+    forall (key: TKey) bag item,
+      MapsTo key bag (ifmap indexed_bag) ->
+      List.In item (benumerate bag) ->
+      E.eq (projection item) key.
+  Proof.
+    intros.
+    destruct indexed_bag as [? consistent].
+    unfold IndexedTreeConsistency in consistent.
+    eapply consistent; eauto.
+  Qed.
+
+  Ltac destruct_if :=
+    match goal with
+        [ |- context [ if ?cond then _ else _ ] ] => destruct cond
+    end.
+
+  Lemma KeyFilter_true :
+    forall {A} k projection (item: A),
+      KeyFilter k projection item = true <-> E.eq (projection item) k.
+  Proof.
+    unfold KeyFilter; intros;
+    destruct_if; intros; intuition.
+  Qed.
+
+  Lemma KeyFilter_false :
+    forall {A} k projection (item: A),
+      KeyFilter k projection item = false <-> ~ E.eq (projection item) k.
+  Proof.
+    unfold KeyFilter; intros;
+    destruct_if; intros; intuition.
+  Qed.
+
+  Definition IndexedBag_bempty 
+             {TBag TItem TBagSearchTerm: Type}
+             {bags_bag: Bag TBag TItem TBagSearchTerm}
+             (projection: TItem -> TKey) :=
+    {| ifmap        := empty TBag;
+       iconsistency := iconsistency_empty projection |}.
+
+  Definition IndexedBag_bstar
+             {TBag TItem TBagSearchTerm: Type}
+             {bags_bag: Bag TBag TItem TBagSearchTerm} :=
+    (@None TKey, @bstar _ _ _ bags_bag).
+
+
+  Definition IndexedBag_bfind_matcher 
+             {TBag TItem TBagSearchTerm: Type}
+             {bags_bag: Bag TBag TItem TBagSearchTerm}
+             (projection: TItem -> TKey)
+             (key_searchterm: (option TKey) * TBagSearchTerm) (item: TItem) :=
+    let (key_option, search_term) := key_searchterm in
+    match key_option with
+      | Some k => KeyFilter k projection item
+      | None   => true 
+    end && (bfind_matcher search_term item).
+
+  Definition IndexedBag_benumerate 
+             {TBag TItem TBagSearchTerm: Type}
+             {bags_bag: Bag TBag TItem TBagSearchTerm}
+             {projection: TItem -> TKey} 
+             (container: @IndexedBag TBag TItem TBagSearchTerm bags_bag projection) :=
+    flatten (List.map benumerate (Values (ifmap container))).
+
+  Definition IndexedBag_bfind
+             {TBag TItem TBagSearchTerm: Type}
+             {bags_bag: Bag TBag TItem TBagSearchTerm}
+             (projection: TItem -> TKey)
+             (container: @IndexedBag TBag TItem TBagSearchTerm bags_bag projection) 
+             (key_searchterm: (option TKey) * TBagSearchTerm) :=
+    let (key_option, search_term) := key_searchterm in
+    match key_option with
+      | Some k =>
+        match find k (ifmap container) with
+          | Some bag => @bfind _ _ _ bags_bag bag search_term
+          | None     => nil
+        end
+      | None   =>
+        flatten (List.map (fun bag =>  @bfind _ _ _ bags_bag bag search_term) (Values (ifmap container)))
+    end.
+
+  Lemma indexed_bag_insert_consistent :
+    forall {TBag TItem TBagSearchTerm: Type}
+           {bags_bag: Bag TBag TItem TBagSearchTerm}
+           {projection: TItem -> TKey} 
+           (container: @IndexedBag TBag TItem TBagSearchTerm bags_bag projection) 
+           (item: TItem),
+      let k := projection item in
+      let fmap := ifmap container in
+      let bag := FindWithDefault k bempty fmap in
+      IndexedTreeConsistency projection (add k (binsert bag item) fmap).
+  Proof.
+    intros.
+
+    intros k' bag' maps_to item'.
+
+    rewrite add_mapsto_iff in maps_to;
+      destruct maps_to as [(is_eq & refreshed) | (neq & maps_to)];
+      subst.
+
+    rewrite (binsert_enumerate item' item bag).
+    intro H; destruct H.
+    apply ((iconsistency container) k' bag); trivial. (* TODO: Why are parens significant here? *)
+
+    rewrite <- is_eq.
+    unfold bag in *.
+
+    unfold fmap in *.
+    destruct (FindWithDefault_dec k (@bempty _ _ _ bags_bag) (ifmap container))
+      as [ [bag' (mapsto & equality)] | (not_found & equality) ];
+      rewrite equality in *; clear equality.
+
+    subst; trivial.
+    exfalso; apply (@benumerate_empty _ _ _ bags_bag) in H; trivial.
+    
+    subst.
+    unfold k in *. 
+    trivial.
+
+    apply ((iconsistency container) k' bag' maps_to item').
+  Qed.    
+
+  Definition IndexedBag_binsert 
+             {TBag TItem TBagSearchTerm: Type}
+             {bags_bag: Bag TBag TItem TBagSearchTerm}
+             (projection: TItem -> TKey)
+             (container: @IndexedBag TBag TItem TBagSearchTerm bags_bag projection) 
+             (item: TItem) : @IndexedBag TBag TItem TBagSearchTerm bags_bag projection :=
+    let k := projection item in
+    let fmap := ifmap container in
+    let bag := FindWithDefault k bempty fmap in
+    {|
+      ifmap := add k (binsert bag item) fmap;
+      iconsistency := indexed_bag_insert_consistent container item
+    |}.
+
+  Lemma IndexedBag_BagInsertEnumerate :
+    forall {TBag TItem TBagSearchTerm: Type}
+           {bags_bag: Bag TBag TItem TBagSearchTerm}
+           (projection: TItem -> TKey),
+      BagInsertEnumerate IndexedBag_benumerate (IndexedBag_binsert projection).
+  Proof.
+
+    unfold BagInsertEnumerate, Values, IndexedBag_benumerate.
+    intros; simpl in *.
+
+    setoid_rewrite in_flatten_iff.
+    setoid_rewrite in_map_iff.
+    setoid_rewrite <- MapsTo_snd.
+
+    split; intro H.
+
+    destruct H as [ items ( in_seq & [ bag (bag_items & [ key maps_to ]) ] ) ].
+    pose proof maps_to as maps_to'.
+    rewrite add_mapsto_iff in maps_to;
+      destruct maps_to as [(is_eq & refreshed) | (neq & maps_to)].
+
+    subst.
+    rewrite (binsert_enumerate _) in in_seq.
+    destruct in_seq as [ in_seq | ? ]; eauto.
+    left.
+    
+    Ltac autoexists :=
+      repeat progress match goal with
+                        | [ |- exists _, _ ] => eexists; autoexists
+                        | [ |- ?a = ?b ]     => first [ (has_evar a; has_evar b; idtac) | eauto]
+                        | [ |- E.eq _ _ ]    => eauto
+                        | [ |- _ /\ _ ]      => split; autoexists
+                        | [ |- _ \/ _ ]      => left; autoexists
+                      end.
+    
+    destruct (FindWithDefault_dec (projection inserted) bempty (ifmap container)) 
+      as [ [result (mapsto & equality)] | (not_found & equality) ];
+      rewrite equality in *; clear equality.
+    
+    autoexists; eauto.
+    
+    exfalso; apply benumerate_empty in in_seq; tauto.
+
+    autoexists; eauto.
+
+    destruct H as [ [ items ( in_seq & [ bag ( bag_items & [ key maps_to ] ) ] ) ] | eq_item_inserted ].
+    
+    pose proof maps_to as maps_to'.
+    apply (iconsistency container) in maps_to.    
+    setoid_rewrite bag_items in maps_to.
+    specialize (maps_to item in_seq).
+    
+    setoid_rewrite add_mapsto_iff.
+
+    destruct (E.eq_dec (projection inserted) key);
+      try solve [ repeat (eexists; split; eauto) ].
+    
+    autoexists.
+
+    apply binsert_enumerate.
+
+    destruct (FindWithDefault_dec (projection inserted) bempty (ifmap container))
+      as [ [bag' (mapsto & equality)] | (not_found & equality) ];
+      rewrite equality in *; clear equality.
+
+    rewrite e in mapsto.
+    pose proof (MapsTo_fun mapsto maps_to') as bag'_bag.
+    rewrite bag'_bag.
+    rewrite bag_items.
+    auto.
+
+    rewrite find_mapsto_iff in maps_to'.
+    rewrite <- e in maps_to'.
+    match goal with 
+      | [ H: ?a = Some ?b, H': ?a = None |- _ ] => assert (Some b = None) by (transitivity a; auto); discriminate
+    end.
+
+    subst item.
+    match goal with
+      | [ |- context [ add ?key ?value ?container ] ] => set (k := key); set (v := value)
+    end.
+
+    exists (benumerate v).
+
+    split.
+
+    unfold v.
+    rewrite (binsert_enumerate _); auto.
+
+    exists v; split; trivial.
+    exists k.
+    apply add_1; trivial.
+  Qed.
+
+  Lemma IndexedBag_BagEnumerateEmpty :
+    forall {TBag TItem TBagSearchTerm: Type}
+           {bags_bag: Bag TBag TItem TBagSearchTerm}
+           (projection: TItem -> TKey),
+      BagEnumerateEmpty IndexedBag_benumerate (IndexedBag_bempty projection).
+  Proof.
+    intros;
+    unfold BagEnumerateEmpty, IndexedBag_benumerate, flatten; simpl;
+    rewrite Values_empty; tauto.
+  Qed.
+
+  Lemma IndexedBag_BagFindStar :
+    forall {TBag TItem TBagSearchTerm: Type}
+           {bags_bag: Bag TBag TItem TBagSearchTerm}
+           (projection: TItem -> TKey),
+      BagFindStar (IndexedBag_bfind projection) IndexedBag_benumerate IndexedBag_bstar.
+  Proof.
+    unfold BagFindStar, IndexedBag_benumerate; simpl.
+    
+    intros; induction (Values (ifmap container)); simpl; trivial.
+    rewrite (@bfind_star _ _ _ bags_bag).
+    f_equal; trivial.
+  Qed.
+
+  Lemma IndexedBag_BagFindCorrect :
+    forall {TBag TItem TBagSearchTerm: Type}
+           {bags_bag: Bag TBag TItem TBagSearchTerm}
+           (projection: TItem -> TKey),
+      BagFindCorrect (IndexedBag_bfind projection)
+                     (IndexedBag_bfind_matcher projection) IndexedBag_benumerate.
+  Proof.
+    intros.
+    destruct search_term as (option_key, search_term).
+    destruct option_key as [ key | ].
+
+    (* Key provided *)
+
+    unfold IndexedBag_benumerate, IndexedBag_bfind_matcher.
+    pose (iconsistency container).
+    unfold IndexedTreeConsistency in i.
+
+    rewrite filter_and'.
+
+    rewrite flatten_filter.
+    
+    Lemma consist :
+      forall 
+        {TBag TItem TSearchTerm bags_bag projection} 
+        (container: @IndexedBag TBag TItem TSearchTerm bags_bag projection),
+      forall k,
+        eq
+          (flatten
+             (List.map (List.filter (KeyFilter k projection))
+                       (List.map benumerate (Values (ifmap container)))))
+          match find k (ifmap container) with
+            | Some bag => benumerate bag
+            | None => nil
+          end.
+    Proof.          
+      intros.
+
+      pose (iconsistency container); unfold IndexedTreeConsistency in i.
+      unfold Values.
+      destruct (find k (ifmap container)) as [ bag | ] eqn:eqfind.
+
+      rewrite <- find_mapsto_iff in eqfind.
+      (* assert (exists k', MapsTo k' bag (ifmap container)) as eqfind' by (exists k; trivial).*)
+
+      pose proof eqfind as maps_to.
+
+      rewrite elements_mapsto_iff in eqfind.
+      apply InA_split in eqfind.
+
+      destruct eqfind as [ l1 [ y [ l2 (y_k_bag & decomp) ] ] ].
+      rewrite decomp.
+      
+      rewrite (map_map snd benumerate).
+      rewrite ! map_app; simpl.
+      
+      pose proof (elements_3w (ifmap container)) as no_dup.
+      rewrite decomp in no_dup; apply NoDupA_swap in no_dup; eauto using equiv_eq_key.
+
+      inversion no_dup as [ | ? ? y_not_in no_dup' ]; subst.
+      rewrite InA_app_iff in y_not_in by eauto using equiv_eq_key.
+      
+      unfold eq_key_elt in y_k_bag; simpl in y_k_bag.
+      destruct y_k_bag as (y_k & y_bag).
+
+      assert (forall k' bag', InA (@eq_key_elt _) (k', bag') (l1 ++ l2) -> 
+                              forall item, 
+                                List.In item (benumerate bag') ->
+                                ~ E.eq (projection item) k).
+      {
+        intros k' bag' in_app item in_bag'_items eq_k.
+
+        rewrite InA_app_iff in in_app; eauto using equiv_eq_key_elt.
+        pose proof in_app as in_app'.
+
+        apply (InA_front_tail_InA _ _ y) in in_app.
+        rewrite <- decomp, <- elements_mapsto_iff in in_app.
+
+        pose proof (i _ _ in_app _ in_bag'_items) as eq_k'. 
+        symmetry in eq_k.
+        pose proof (E.eq_trans eq_k eq_k').
+
+        assert (eq_key y (k', bag')) as y_eq by (unfold eq_key; simpl; eauto).
+
+        destruct in_app' as [ in_seq | in_seq ];
+          (apply (InA_eqke_eqk (k2 := fst y) (snd y)) in in_seq; eauto);
+          rewrite <- surjective_pairing in in_seq; intuition.
+      }
+
+      Lemma In_InA :
+        forall (A : Type) (l : list A) (eqA : relation A) (x : A),
+          Equivalence eqA -> List.In x l -> InA eqA x l.
+      Proof.
+        induction l; intros; simpl in *.
+        exfalso; eauto using in_nil.
+        destruct H0.
+        apply InA_cons_hd; subst; reflexivity.
+        apply InA_cons_tl, IHl; trivial.
+      Qed.
+
+      rewrite ! map_filter_all_false;
+        [ | intros subseq in_map item in_subseq;
+            rewrite in_map_iff in in_map;
+            destruct in_map as [ (k', bag') (benum_eq & in_seq) ];
+            rewrite KeyFilter_false;
+            
+            simpl in benum_eq;
+            subst subseq;
+            apply (H k' bag'); 
+            eauto;
+            
+            apply In_InA; eauto using equiv_eq_key_elt;
+            rewrite in_app_iff;
+            eauto 
+              .. ].
+
+      rewrite 
+        flatten_app, 
+      flatten_head, 
+      !flatten_nils, 
+      app_nil_l, app_nil_r, 
+      <- y_bag,
+      filter_all_true; trivial.
+
+      intros;
+        rewrite KeyFilter_true;
+        apply (iconsistency container _ bag); eauto.
+
+      Lemma nil_in_false :
+        forall {A} seq,
+          seq = nil <-> ~ exists (x: A), List.In x seq.
+      Proof.
+        split; intro H.
+        intros [ x in_seq ]; subst; eauto using in_nil.
+        destruct seq as [ | a ]; trivial.
+        exfalso; apply H; exists a; simpl; intuition.
+      Qed.
+      
+      rewrite nil_in_false.
+      intros [item item_in].
+
+      rewrite in_flatten_iff in item_in.
+      do 2 setoid_rewrite in_map_iff in item_in.
+
+      destruct item_in as 
+          [ subseq 
+              (in_subseq 
+                 & [ subseq_prefilter 
+                       ( pre_post_filter 
+                           & [ bag 
+                                 (eq_bag_pre_filter 
+                                    & bag_in) ] ) ] ) ].
+
+      subst subseq.
+      rewrite filter_In in in_subseq.
+      destruct in_subseq as (in_subseq_prefilter & key_filter).
+
+      rewrite KeyFilter_true in key_filter.
+      rewrite <- MapsTo_snd in bag_in.
+      destruct bag_in as [k' maps_to].
+
+      subst.
+      rewrite <- key_filter in eqfind.
+      rewrite <- (iconsistency container k' bag maps_to _ in_subseq_prefilter) in maps_to.
+      rewrite find_mapsto_iff in maps_to.
+
+      congruence.
+    Qed.
+
+    simpl.
+    rewrite consist.
+    destruct (find key (ifmap container)) as [ bag | ].
+
+    apply bfind_correct.
+    eauto using SetEq_Reflexive.
+
+    (* No key provided *)
+
+    simpl. unfold IndexedBag_benumerate, IndexedBag_bfind_matcher.
+    rewrite flatten_filter.
+
+    induction (Values (ifmap container)); simpl.
+
+    compute; tauto.
+
+    rewrite IHl.
+
+    Lemma SetEq_app :
+      forall {A: Type} (s1 t1 s2 t2: list A),
+        (SetEq s1 s2) /\ (SetEq t1 t2) -> SetEq (s1 ++ t1) (s2 ++ t2).
+    Proof.
+      unfold SetEq; 
+      intros A s1 t1 s2 t2 (s1s2 & t1t2); 
+      split;
+      rewrite ! in_app_iff;
+      intro inApp;
+      [ rewrite s1s2, t1t2 in inApp
+      | rewrite <- s1s2, <- t1t2 in inApp ];
+      trivial.
+    Qed.
+
+    apply SetEq_app; split; eauto using SetEq_Reflexive.
+    apply bfind_correct.
+  Qed.
+  
+  Instance IndexedBagAsBag 
+           (TBag TItem TBagSearchTerm: Type) 
+           (bags_bag: Bag TBag TItem TBagSearchTerm) (projection: TItem -> TKey) 
+  : Bag 
+      (@IndexedBag TBag TItem TBagSearchTerm bags_bag projection) 
+      TItem 
+      ((option TKey) * TBagSearchTerm) :=
+    {| 
+      bempty        := IndexedBag_bempty projection;
+      bstar         := IndexedBag_bstar;
+      bfind_matcher := IndexedBag_bfind_matcher projection;
+
+      benumerate := IndexedBag_benumerate;
+      bfind      := IndexedBag_bfind projection;
+      binsert    := IndexedBag_binsert projection;
+
+      binsert_enumerate := IndexedBag_BagInsertEnumerate projection;
+      benumerate_empty  := IndexedBag_BagEnumerateEmpty projection;
+      bfind_star        := IndexedBag_BagFindStar projection;
+      bfind_correct     := IndexedBag_BagFindCorrect projection
+    |}. 
+End TreeBag.
