ADTExamples/QueryStructure/ProcessScheduler/SetEqProperties.v
@@ -1,0 +1,181 @@
+Require Import SetEq Setoid AdditionalLemmas List.
+
+Definition IsSetEqSafe {A B: Type} (proc: list A -> list B) :=
+  forall (seq1 seq2: list A),
+    SetEq seq1 seq2 ->
+    SetEq (proc seq1) (proc seq2).
+
+Lemma SetEq_modulo_SetEqSafe_fun :
+  forall {A B: Type},
+  forall (seq1: list B) (seq2 seq3: list A),
+  forall (proc: list A -> list B),
+    SetEq seq2 seq3 ->
+    IsSetEqSafe proc ->
+    (SetEq seq1 (proc seq2) <-> SetEq seq1 (proc seq3)).
+Proof.
+  intros; eauto using SetEq_trans_iff_2.
+Qed.
+
+Lemma SetEq_after_map :
+  forall {A B: Type} (seq1 seq2: list A),
+  forall (proc: A -> B),
+    SetEq seq1 seq2 -> SetEq (map proc seq1) (map proc seq2).
+Proof.
+  intros ? ? ? ? ? set_eq;
+  unfold SetEq in *;
+  intro x;
+  split;
+  intros in_map;
+  rewrite in_map_iff in in_map;
+  destruct in_map as [pred (is_pred, pred_in_list)];
+  specialize (set_eq pred);
+  subst;
+  intuition;
+  eauto using in_map.
+Qed.
+
+Lemma map_modulo_SetEq :
+  forall {A B: Type} (seq1 seq1': list A) (seq2: list B),
+  forall (proc: A -> B),
+    SetEq seq1 seq1' ->
+    (SetEq (map proc seq1) (seq2) <-> SetEq (map proc seq1') (seq2)).
+Proof.
+  intros;
+  simpl;
+  apply SetEq_trans_iff;
+  apply SetEq_after_map;
+  trivial.
+Qed.
+
+Lemma IsSetEqSafe_map :
+  forall {A B: Type} (proc: A -> B),
+    IsSetEqSafe (fun x => List.map proc x).
+Proof.
+  unfold IsSetEqSafe;
+  eauto using SetEq_after_map.
+Qed.
+
+Lemma IsSetEqSafe_filter :
+  forall {A: Type} (pred: A -> bool),
+    IsSetEqSafe (fun x => List.filter pred x).
+Proof.
+  unfold IsSetEqSafe, SetEq;
+  intros;
+  repeat rewrite filter_In;
+  specialize (H x);
+  intuition.
+Qed.
+
+Add Parametric Relation (A: Type) : (list A) (@SetEq A)
+    reflexivity proved by SetEq_Reflexive
+    symmetry proved by SetEq_Symmetric
+    transitivity proved by SetEq_Transitive
+      as set_eq.
+
+Add Parametric Morphism {A: Type} (x: A) :
+  (List.In x)
+    with signature (@SetEq A ==> iff)
+      as in_morphism.
+Proof.
+  intros s1 s2;
+  unfold SetEq;
+  intros;
+  eauto.
+Qed.
+
+Add Parametric Morphism {A B: Type} (proc: A -> B) :
+  (List.map proc)
+    with signature (@SetEq A ==> @SetEq B)
+      as map_morphism.
+Proof.
+  apply IsSetEqSafe_map.
+Qed.
+
+Add Parametric Morphism {A: Type} (pred: A -> bool) :
+  (List.filter pred)
+    with signature (@SetEq A ==> @SetEq A)
+      as filter_morphism.
+Proof.
+  apply IsSetEqSafe_filter.
+Qed.
+
+Require Import EnsembleListEquivalence.
+
+Add Parametric Morphism {A: Type} (ens: A -> Prop) :
+  (EnsembleListEquivalence ens)
+    with signature (@SetEq A ==> @iff)
+      as ensemble_list_equivalence_morphism.
+Proof.
+  firstorder.
+Qed.
+
+Add Parametric Morphism {A: Type} :
+  flatten
+    with signature (@SetEq (list A) ==> @SetEq A)
+      as concat_right_morphism.
+Proof.
+  unfold SetEq;
+  setoid_rewrite in_flatten_iff;
+  firstorder.
+Qed.
+
+(*
+Require Import State.
+
+Add Parametric Morphism (A: Type) :
+  (State_rect (fun _ => list A))
+    with signature (@SetEq A ==> @SetEq A ==> pointwise_relation _ (@SetEq A))
+      as rect_morphism.
+Proof.
+  intros;
+  unfold pointwise_relation, State_rect;
+  intro state; destruct state; trivial.
+Qed.
+*)
+
+Add Parametric Morphism {A: Type} : (@SetUnion A)
+    with signature (@SetEq A ==> @SetEq A ==> @SetEq A)
+      as union_morphism.
+Proof.
+  unfold SetEq, SetUnion;
+  intros;
+  rewrite ! in_app_iff;
+  intuition;
+  repeat match goal with
+           | [ H: List.In ?x _, H': forall _, _ |- _ ] => try specialize (H' x)
+         end;
+  tauto.
+Qed.
+
+Lemma SetEq_append : (* TODO: Rename to cons *)
+  forall {A: Type} (seq1 seq2: list A) (x: A),
+    SetEq seq1 seq2 -> SetEq (x :: seq1) (x :: seq2).
+Proof.
+  intros A s1 s2 x s_eq;
+  unfold SetEq;
+  split; intro H;
+  simpl in *;
+  [rewrite s_eq in H | rewrite <- s_eq in H];
+  intuition.
+Qed.
+
+Lemma seteq_nil_nil :
+  forall {A} seq,
+    @SetEq A seq nil <-> seq = nil.
+Proof.
+  unfold SetEq.
+  intros; destruct seq.
+
+  tauto.
+  split; [ | discriminate ].
+  intro H; specialize (H a).
+  exfalso; simpl in H; rewrite <- H; eauto.
+Qed.
+
+Lemma seteq_nil_nil' :
+  forall {A} seq,
+    @SetEq A nil seq <-> seq = nil.
+Proof.
+  setoid_rewrite SetEq_Symmetric_iff.
+  intro; exact seteq_nil_nil.
+Qed.
